---
title: "Tarea7"
author: "Carlos GÃ¡lvez"
date: "5/23/2020"
output:
  pdf_document: default
  html_document: default
---

```{r setup, include=FALSE}
knitr::opts_chunk$set(echo = TRUE)
```

1.

A1)
$$
A_{1} = \begin{pmatrix}1 & 4 & 6\\2 & -1 & 3 \\ 3 & 2 & 5\end{pmatrix}\\
$$
$$
U = A \tilde{}F_{2} - 2F_{1}\begin{pmatrix}1 & 4 & 6\\0 & -9 & -9 \\ 3 & 2 & 5\end{pmatrix} \tilde{} F_{3} - 3F_{1}\begin{pmatrix}1 & 4 & 6\\0 & -9 & -9 \\ 0 & -10 & -13\end{pmatrix} \tilde{} -\frac{1}{9}F_{2} = 
$$
$$= \begin{pmatrix}1 & 4 & 6\\0 & 1 & 1 \\ 0 & -10 & -13\end{pmatrix} \tilde{} F_{3} + 10F_{2} \begin{pmatrix}1 & 4 & 6\\0 & 1 & 1 \\ 0 & 0 & -3\end{pmatrix} 
\tilde{}-\frac{1}{3}F_{3} \begin{pmatrix}1 & 4 & 6\\0 & 1 & 1 \\ 0 & 0 & 1\end{pmatrix}
$$

$$
U = F_{3} (-\frac{1}{3}) \cdot F_{32}(10) \cdot F_{2}(-\frac{1}{9}) \cdot F_{31}(-3) \cdot F_{21}(-2)\cdot A_{1}
$$

$$
L = F_{21}(2) \cdot F_{31}(3) \cdot F_{2}(-9)\cdot F_{32}(-10) \cdot F_{3}(-3)
$$

$$L = \begin{pmatrix}1 & 0 & 0\\2 & 1 & 0 \\ 0 & 0 & 1\end{pmatrix} \cdot \begin{pmatrix}1 & 0 & 0\\0 & 1 & 0 \\ 3 & 0 & 1\end{pmatrix} \cdot \begin{pmatrix}1 & 0 & 0\\0 & -9 & 0 \\ 0 & 0 & 1\end{pmatrix} \cdot \begin{pmatrix}1 & 0 & 0\\0 & 1 & 0 \\ 0 & -10 & 1\end{pmatrix} \cdot \begin{pmatrix}1 & 0 & 0\\0 & 1 & 0 \\ 0 & 0 & -3\end{pmatrix}$$
$$= \begin{pmatrix}1 & 0 & 0\\2 & 1 & 0 \\ 3 & 0 & 1\end{pmatrix} \cdot \begin{pmatrix}1 & 0 & 0\\0 & -9 & 0 \\ 0 & -10 & 1\end{pmatrix} \cdot \begin{pmatrix}1 & 0 & 0\\0 &1 & 0 \\ 0 & 0 & -3\end{pmatrix} = \\=\begin{pmatrix}1 & 0 & 0\\2 & -9 & 0 \\ 3 & -10 & 1\end{pmatrix} \cdot\begin{pmatrix}1 & 0 & 0\\0 & 1 & 0 \\ 0 & 0 & -3\end{pmatrix} = \begin{pmatrix}1 & 0 & 0\\2 & -9 & 0 \\ 3 & -10 & -3\end{pmatrix}$$

A2)
$$
A_{2} = \begin{pmatrix}2 & 4 & 2\\1 & 3 & 1 \\ 7 & 5 & 6\end{pmatrix} \\
U = A  \tilde{} F_{2} - F_{1} \begin{pmatrix}1 & 3 & 1 \\2 & 4 & 2\\ 7 & 5 & 6\end{pmatrix} \tilde{} F_{2}-2F_{1} \begin{pmatrix}1 & 3 & 1 \\0 & -2 & 0\\ 7 & 5 & 6\end{pmatrix} \\\tilde{} F_{3} - 7F_{1}\\
\begin{pmatrix}1 & 3 & 1 \\0 & -2 & 0\\ 0 & -16 & -1\end{pmatrix} \tilde{} -\frac{1}{2}F_{2} \begin{pmatrix}1 & 3 & 1 \\0 & 1 & 0\\ 0 & -16 & -1\end{pmatrix} \\\tilde{} F_{3} + 16F_{2} \begin{pmatrix}1 & 3 & 1 \\0 & 1 & 0\\ 0 & 0 & -1\end{pmatrix} \tilde{} -1F_{3} = \begin{pmatrix}1 & 3 & 1 \\0 & 1 & 0\\ 0 & 0 & 1\end{pmatrix} \\
P = F_{12} = \begin{pmatrix}0 & 1 & 0 \\1 & 0 & 0\\ 0 & 0 & 1\end{pmatrix}
$$
$$
U = F_{3}(-1)\cdot F_{32}(16)\cdot F_{2}(-\frac{1}{2})\cdot F_{31}(-7)\cdot F_{21}(-2)\cdot PA\\
L = F_{21}(2)\cdot F_{31}(7)\cdot F_{2}(-2)\cdot F_{32}(-16)\cdot F_3(-1) = \\
= \begin{pmatrix}1 & 0 &0 \\2 & 1 & 0\\ 0 & 0 & 1\end{pmatrix} \cdot \begin{pmatrix}1 & 0 &0 \\0 & 1 & 0\\ 7 & 0 & 1\end{pmatrix} \cdot \begin{pmatrix}1 & 0 &0 \\0 & -2 & 0\\ 0 & 0 & 1\end{pmatrix} \cdot \begin{pmatrix}1 & 0 &0 \\0 & 1 & 0\\ 0 & -16 & 1\end{pmatrix} \cdot \begin{pmatrix}1 & 0 &0 \\0 & 1 & 0\\ 0 & 0 & -1\end{pmatrix} = \\
\begin{pmatrix}1 & 0 &0 \\2 & 1 & 0\\ 7 & 0 & 1\end{pmatrix} \cdot \begin{pmatrix}1 & 0 &0 \\0 & -2 & 0\\ 0 & -16 & 1\end{pmatrix} \cdot \begin{pmatrix}1 & 0 &0 \\0 & 1 & 0\\ 0 & 0 & -1\end{pmatrix} =\\
=\begin{pmatrix}1 & 0 &0 \\2 & -2 & 0\\ 7 & -16 & 1\end{pmatrix} \cdot \begin{pmatrix}1 & 0 &0 \\0 & 1 & 0\\ 0 & 0 & -1\end{pmatrix} = \begin{pmatrix}1 & 0 &0 \\2 & -2 & 0\\ 7 & -16 & -1\end{pmatrix}
$$

A3)

$$
A_3 = \begin{pmatrix}0 & 0 & 5\\-1 & 4 & 1\\2 & -3 & 2\end{pmatrix}
$$

$$ 
U = A \tilde{} F_3 - F_1 \begin{pmatrix}2 & -3 & 2\\-1 & 4 & 1\\0 & 0 & 5\end{pmatrix} \tilde{}\frac{1}{2}F_1 \begin{pmatrix}1 & \frac{-3}{2} & 1\\-1 & 4 & 1\\0 & 0 & 5\end{pmatrix} \tilde{}F_2+1F_1 \begin{pmatrix}1 & \frac{-3}{2} & 1\\0 & \frac{5}{2} & 2\\0 & 0 & 5\end{pmatrix}\tilde{}\frac{2}{5}F_2\\\begin{pmatrix}1 & \frac{-3}{2} & 1\\0 & 1 & \frac{4}{5}\\0 & 0 & 5\end{pmatrix}\tilde{}\frac{1}{5}F_3\begin{pmatrix}1 & \frac{-3}{2} & 1\\0 & 1 & \frac{4}{5}\\0 & 0 & 1\end{pmatrix}
$$

$$
P = F_{13} = \begin{pmatrix}0 & 0 & 1\\0 & 1 & 0\\1 & 0 & 0\end{pmatrix}
$$

$$
U = F_3(\frac{1}{5}) \cdot F_2(\frac{2}{5})\cdot F_{21}(1)\cdot F_1(\frac{1}{2}) \cdot PA
$$



$$
L = F_1(2)\cdot F_{21}(-1)\cdot F_2(\frac{5}{2})\cdot F_{3}(5) =\\
= \begin{pmatrix}2 & 0 & 0\\0 & 1 & 0\\0 & 0 & 1\end{pmatrix} \cdot \begin{pmatrix}1 & 0 & 0\\-1 & 1 & 0\\0 & 0 & 1\end{pmatrix} \cdot \begin{pmatrix}1 & 0 & 0\\0 & \frac{5}{2} & 0\\0 & 0 & 1\end{pmatrix} \cdot \begin{pmatrix}1 & 0 & 0\\0 & 1 & 0\\0 & 0 & 5\end{pmatrix} = \begin{pmatrix}2 & -0 & 0\\-1 & 1 & 0\\0 & 0 & 1\end{pmatrix} \cdot \begin{pmatrix}1 & 0 & 0\\0 & \frac{5}{2} & 0\\0 & 0 & 5\end{pmatrix} = \begin{pmatrix}2 & 0 & 0\\-1 & \frac{5}{2} & 0\\0 & 0 & 5\end{pmatrix}\\ \tilde{}F_3-\frac{2}{7}F_2\begin{pmatrix}\end{pmatrix}\tilde{}\frac{1}{21}F_2
$$

A4)
$$
A_4 = \begin{pmatrix}3&9&-2 \\ 6&-3&8  \\ 4&6&5\end{pmatrix}
$$
$$
U = A \tilde{} F_2-2F_1 \begin{pmatrix}3&9&-2 \\0&-21&12\\4&6&5\end{pmatrix}\tilde{}\frac{1}{3}F_1\begin{pmatrix}1&3&-\frac{2}{3}\\0&-21&12\\4&6&5\end{pmatrix}\tilde{}F_3-4F_1\begin{pmatrix}1&3&-\frac{2}{3}\\0&-21&12\\0&-6&\frac{23}{3}\end{pmatrix}\\
\tilde{}F_3 - \frac{2}{7}F_2\begin{pmatrix}1&3&-\frac{2}{3}\\0&-21&12\\0&0&\frac{89}{21}\end{pmatrix}\tilde{}-\frac{1}{21}F_2\begin{pmatrix}1&3&-\frac{2}{3}\\0&1&-\frac{4}{7}\\0&0&\frac{89}{21}\end{pmatrix}\tilde{}\frac{21}{89}F_3\begin{pmatrix}1&3&-\frac{2}{3}\\0&1&-\frac{4}{7}\\0&0&1\end{pmatrix}
$$

$$
U = F_3(\frac{21}{89})\cdot F_2(-\frac{1}{21})\cdot F_{32}(-\frac{2}{7})\cdot F_{31}(-4)\cdot F_1(\frac{1}{3})\cdot F_{21}(-2) \cdot A 
$$
$$
L = F_{21}(2)\cdot F_1(3)\cdot F_{31}(4)\cdot F_{32}(\frac{2}{7})\cdot F_2(-21)\cdot F_3(\frac{89}{21}) =\\=\begin{pmatrix}1&0&0\\2&1&0\\0&0&1\end{pmatrix}\cdot\begin{pmatrix}3&0&0\\0&1&0\\0&0&1\end{pmatrix}\cdot\begin{pmatrix}1&0&0\\0&1&0\\4&0&1\end{pmatrix}\cdot \begin{pmatrix}1&0&0\\0&1&0\\0&\frac{2}{7}&1\end{pmatrix}\cdot \begin{pmatrix}1&0&0\\0&-21&0\\0&0&1\end{pmatrix}\cdot \begin{pmatrix}1&0&0\\0&1&0\\0&0&\frac{89}{21}\end{pmatrix} = \\
=\begin{pmatrix}3&0&0\\6&1&0\\0&0&1\end{pmatrix}\cdot \begin{pmatrix}1&0&0\\0&1&0\\4&\frac{2}{7}&1\end{pmatrix}\cdot \begin{pmatrix}1&0&0\\0&-21&0\\0&0&\frac{89}{21}\end{pmatrix} = \begin{pmatrix}3&0&0\\6&-21&0\\4&-6&\frac{89}{21}\end{pmatrix}
$$
2.
$$
PAX = PB\\
LUX = PB\\
UX = Y\\
LY = PB
$$
B1)
$$
AX = B\\
LUX = B\\
UX = Y\\
LY = B\\ 
\begin{pmatrix}1&0&0\\2&-9&0\\3&-10&-3\end{pmatrix} \cdot \begin{pmatrix}y_1\\y_2\\y_3\end{pmatrix} = \begin{pmatrix}-1\\7\\2\end{pmatrix}
$$
$$
y_1 = -1;\\
2y_1-9y_2 = 7\\
-2 -9y_2 = 7\\
-9y_2 = 9\\
y_2 = \frac{9}{-9} = -1;\\
3y_1-10y_2-3y_3=2\\
-3+10-3y_3 = 2\\
-3y_3 = -5\\
y_3 = \frac{-5}{-3} = \frac{5}{3};
$$
$$
UX = B = \begin{pmatrix}1&4&6\\0&1&1\\0&0&1\end{pmatrix}\cdot\begin{pmatrix}x_1\\x_2\\x_3\end{pmatrix} =  \begin{pmatrix}-1\\-1\\\frac{5}{3}\end{pmatrix}\\
x_3 = \frac{5}{3};\\
x_2 + x_3 = -1\\
x_2 = -1 - \frac{5}{3}= -\frac{8}{3};\\
x_1 + 4(-\frac{8}{3})+ 6(\frac{5}{3}) = -1\\
x_1 = -1 + \frac{32}{3} - 10 = -\frac{1}{3}
$$
B2)
$$
AX = B\\
LUX = B\\
UX = Y\\
LY = B 
$$
$B = \begin{pmatrix}6\\1\\1\end{pmatrix}$
$$
\begin{pmatrix}2&0&0\\1&1&0\\7&-9&-1\end{pmatrix}\cdot \begin{pmatrix}y_1\\y_2\\y_3\end{pmatrix}=\begin{pmatrix}6\\1\\1\end{pmatrix}\\
y_1 = \frac{6}{2}=3;\\
y_1 + y_2 = 1\\
3 + y_2 = 1\\
y_2 = 1-3 = -2;\\
7y_1 - 9y_2 - 6y_3 = 1\\
21 - 18 - y_3 = 1\\
-y_3 = 1 - 21 + 18\\
y_3 = \frac{-38}{-1} = 38;
$$

B3)
$$
LY = PB\\
\begin{pmatrix}2&0&0\\-1& \frac{5}{2}&0\\0&0&5\end{pmatrix}\cdot \begin{pmatrix}y_1\\y_2\\y_3\end{pmatrix} = \begin{pmatrix}0&0&1\\0&1&0\\1&0&0\end{pmatrix}\cdot\begin{pmatrix}3\\10\\4\end{pmatrix} = \begin{pmatrix}4\\10\\3\end{pmatrix}\\
y_1 = \frac{4}{2} = 2;\\
-1y_1+\frac{5}{2}\cdot y_2 = 10\\
y_2 = \frac{10 + 2}{\frac{5}{2}} = \frac{24}{5};\\
y_3 = \frac{3}{5};\\
$$
$$
UX = Y\\
\begin{pmatrix}1&-\frac{3}{2}&1\\0&1&\frac{4}{5}\\0&0&1\end{pmatrix}\cdot\begin{pmatrix}x_1\\x_2\\x_3\end{pmatrix} = \begin{pmatrix}2\\\frac{24}{5}\\\frac{3}{5}\end{pmatrix}\\
x_3=\frac{3}{5};\\
x_2=\frac{24}{5}-\frac{4}{5}\cdot \frac{3}{5}= \frac{120}{25}-\frac{12}{25} = \frac{108}{25};\\
x_1-\frac{3}{2}x_2+x_3=2\\
x_1 + (-\frac{3}{2}\cdot\frac{108}{25}) + \frac{3}{5}  = 2 
x_1 = 2 - \frac{3}{5} + \frac{324}{50} = \frac{50}{25} - \frac{15}{25} + \frac{162}{25} = \frac{197}{25}
$$
B4)
$$
LY = B
\begin{pmatrix}3&0&0\\6&-21&0\\4&-6&\frac{89}{21}\end{pmatrix}\cdot\begin{pmatrix}y_1\\y_2\\y_3\end{pmatrix}=\begin{pmatrix}-1\\0\\2\end{pmatrix}\\
y_1 = -\frac{1}{3};\\
6y_1-21y_2 = 0\\
y_2 = -\frac{2}{21};\\
4y_1-6y_2+\frac{89}{21}y_3 = 2\\
-\frac{4}{3}+\frac{4}{7}+\frac{89}{21}y_3 = 2\\
y_3 = \frac{2 + \frac{4}{3}-\frac{4}{7}}{\frac{89}{21}} = \frac{\frac{42}{21} + \frac{28}{21}-\frac{12}{21}}{\frac{89}{21}} = \frac{\frac{58}{21}}{\frac{89}{21}} = \frac{58}{89};
$$


$$
UX = Y\\
\begin{pmatrix}1&3&-\frac{3}{2}\\0&1&-\frac{4}{7}\\0&0&1\end{pmatrix}\cdot\begin{pmatrix}x_1\\x_2\\x_3\end{pmatrix} = \begin{pmatrix}-\frac{1}{3}\\-\frac{2}{21}\\\frac{58}{89}\end{pmatrix}\\
x_3 = \frac{58}{89};\\
x_2 -\frac{4}{7}x_3 = -\frac{2}{21}\\
x_2 -\frac{4}{7}\cdot\frac{58}{89}= -\frac{2}{21}\\
x_2 = -\frac{2}{21}+\frac{232}{623} = \frac{3626}{13083} = \frac{74}{267};\\
x_1 + 3x_2 -\frac{3}{2}x_3 = -\frac{1}{3}\\
x_1 + 3\cdot \frac{74}{267} - \frac{2}{3}\cdot\frac{58}{89} = -\frac{1}{3}\\
x_1 + \frac{222}{267} - \frac{116}{267} = -\frac{1}{3}\\
x_1 = -\frac{1}{3} - \frac{106}{267} = -\frac{89}{267} - \frac{106}{267} = \frac{-195}{267} = \frac{-65}{89}
$$
3.
$$A = \begin{pmatrix}1 & 1 &|&-2\\1 & 2 &|&-1\\-&-&|&--\\0 & 0 &|&2\end{pmatrix} = \begin{pmatrix}B &|&C\\--&|&--\\0 & |& D\end{pmatrix}$$


$$A^{-1} = \begin{pmatrix}B^{-1} &|&-B^{-1}CD^{-1}\\--&|&------\\0 & |& D^{-1}\end{pmatrix}$$
$$det(B) = 1\cdot2 - 1\cdot1 = 1\\
det(D) = 2\\
\begin{pmatrix}1&1&|&1&0\\1&2&|&0&1\end{pmatrix}\tilde{}F_2-F_1\\\begin{pmatrix}1&1&|&1&0\\0&1&|&-1&1\end{pmatrix} \tilde{}F_1-F_2\\
\begin{pmatrix}1&0&|&2&-1\\0&1&|&-1&1\end{pmatrix}\\
B^{-1} = \begin{pmatrix}2&-1\\-1&1\end{pmatrix}\\
D^{-1} = \frac{1}{2}\\
-B^{-1}\cdot C = \begin{pmatrix}-2&1\\1&-1\end{pmatrix} \cdot \begin{pmatrix}-2\\-1\end{pmatrix} = \begin{pmatrix}3\\-1\end{pmatrix}\\
-B^{-1}CD^{-1} = \begin{pmatrix}3\\-1\end{pmatrix}\cdot\begin{pmatrix}\frac{1}{2}\end{pmatrix} = \begin{pmatrix}\frac{3}{2}\\-\frac{1}{2}\end{pmatrix}\\
A^{-1} = \begin{pmatrix}2&-1&\frac{3}{2}\\-1&-1&-\frac{1}{2}\\0&0&\frac{1}{2}\end{pmatrix}$$